$\displaystyle{等式x^2 - x -2 = 0}$
$$\begin{aligned}
& x^2 - x -2 = 0 \\
& x^2 -x + \frac{1}{4} = 2 + \frac{1}{4} \\
& (x-\frac{1}{2})^2 = \frac{9}{4} \\
& x- \frac{1}{2}  = \frac{3 }{2} \\
& x =\frac{1}{2} \pm \frac{3}{2} \\
& x = \begin{cases} &2 \\ &-1 \\ \end{cases}
\end{aligned}$$

## 求根公式推导
$\displaystyle{ax^2 + bx + c = 0}$
$$\begin{aligned}
& x^2 + \frac{b}{a }x + \frac{c}{a } = 0 \\
& x^2 + \frac{b}{a }x + (\frac{b}{2a })^2  = (\frac{b}{2a})^2 - \frac{c}{a} \\
& (x+\frac{b}{2a})^2  = \frac{b^2}{4a^2} - \frac{4ac}{4a^2}\\
& x + \frac{b}{2a} = \frac{\pm \sqrt{b^2 - 4ac}}{\pm2a}   \\
& x = \frac{-b \pm \sqrt{b^2 - 4ac}}{2a}
\end{aligned}$$


## 十字相乘法
$\displaystyle{ax^2 + bx + c = 0}$

$$\begin{aligned}
& set \quad a = x_0 \cdot  y_0 ,\\
&c = x_1 \cdot y_1 ,\\
&b = x_0 \cdot y_1 + x_1 \cdot  y_0\\
\end{aligned}$$

$\displaystyle{x^2 - x -2 = 0}$
$$\begin{aligned}
& 一般a = 1的情况下，即x_0 = x , y_0 = x，先确定c的式子\\
& 即b = -1 = x+y \\
&  c = -2 = x*y\\
& \therefore x=-2 ,y  =1\\
& (x-2)(x+1) = 0 \\
\end{aligned}$$

$\displaystyle{x^2 - 10x + 16 = 0}$
$$\begin{aligned}
& \because a= 1\\
& \therefore x+y = -10 , xy = 16 \\
& \therefore x = -2 , y = -8 \\
& (x-2)(x-8) = 0 \\
\end{aligned}$$


## 因式分解
$\displaystyle{化简x^3 + y^3}$
$$\begin{aligned}
& x^3 + y^3 = x^3 + x^2y - x^2y + y^3 + xy^2 - xy^2 \\
& = x^3 + x^2y - xy^2 + y^3 + xy^2 - x^2y \\
& = x^3 - x^2y + xy^2 + y^3 - xy^2 + x^2y\\
& = x(x^2-xy + y^2) + y(y^2 - xy + x^2) \\
& = (x+y)(x^2 - xy + y^2)
\end{aligned}$$

$\displaystyle{化简(x+y)^3}$
$$\begin{aligned}
& (x+y)^3 = (x+y)(x+y)^2 \\
& =(x+y)(x^2 + 2xy + y^2) = x^3 + 2x^2y + xy^2 + x^2y + 2xy^2 + y^3 \\
& = x^3 + 3x^2y + 3xy^2 + y^3\\
\end{aligned}$$

