### 选择题
>1.
$$\begin{aligned}
& A \quad  if \quad x = -1 \\
& B \quad  if \quad x = -1\\
& D \quad  if \quad x = 1 \\
\end{aligned}$$
>2.
$$\begin{aligned}
& f(x) = \frac{x-1}{x} =>  y = \frac{x-1}{x} = > xy = x-1 => x(y-1) = -1 => x =  \frac{1}{1-y} \\
& \therefore f^{-1}(x) = \frac{1}{1-x} \\
& f^{-1}(x+1) = \frac{1}{1- (x+1)} = -\frac{1}{x} \\
\end{aligned}$$
>3.
$$\begin{aligned}
& A \quad if \quad U_n = -1 \\
& B \quad if \quad y_n = \frac{1}{n} ,x_n = n \\
& C \quad if \quad x_n = 1 + (-1)^n ,y_n = 1 - (-1)^n ,then \quad no \quad exitst \\
\end{aligned}$$
>4.
$$\begin{aligned}
& \lim\limits_{x\rightarrow 0^-}f(x) = 1+x^2 = 1 \\
& \lim\limits_{x\rightarrow 0^+}f(x)=  2x -1 = -1 \\
& \lim\limits_{x\rightarrow 0}f(x) =>no \quad exitst \\
\end{aligned}$$
>5.
$$\begin{aligned}
& A \quad if \quad f(x) = x^2 + 1 , \phi(x) = \begin{cases} &2,x<1 \\ &-2,x\geq 1 \\ \end{cases} ,then\quad \phi(f(x)) = -2\\
& B \quad if \quad 同上[\pm 2]^2 =  4 \\
& C \quad if \quad 同上f(x)为连续函数 \\
& D \quad \because f(x)连续,\phi(x)间断 \therefore f(x) \cdot \frac{\phi(x)}{f(x)}  = \phi(x) => 连续 * 间断 = 间断\\
\end{aligned}$$
>6.
$$\begin{aligned}
&\lim\limits_{x\rightarrow 0^-}e^x = \lim\limits_{x\rightarrow 0^+}a+x+2 = 1 \\
& a + 0 + 2=  1  ,a = -1 \\
\end{aligned}$$
>7.
$$\begin{aligned}
& 0 \leq \ln{(x+1)} < 1 \\
& 0 \leq  \ln{(x+1)} => x+1 \geq 1 => x \geq 0 \\
& \ln{(x+1)} < 1 => 0< x+1 < e => -1 < x < e-1  \\
& \therefore  [0,e-1)\\
\end{aligned}$$
>8.
 $$\begin{aligned}
& if \quad x < 0 , g(x^2) = x^2+2 \\
& if \quad x \geq 0,g(-x) = 2+x \\
& \begin{cases} &x^2+2 , x<0 \\ &2+x , x\geq 0 \\ \end{cases} \\
\end{aligned}$$

>9.
$$\begin{aligned}
& \lim\limits_{x\rightarrow 2}f(x) = \infty  \\
& \therefore 第二类间断点 \\
\end{aligned}$$

>10.
$$\begin{aligned}
& 无穷小量=> \lim\limits_{x\rightarrow 0}(\sin{2x} - 2\sin{x})\\
& \sin{2x}- 2\sin{x} = 2\sin{x}\cos{x} - 2\sin{x} = 2\sin{x}(\cos{x} - 1) = -2\sin{x}(1 - \cos{x}) \\
&  = \lim\limits_{x\rightarrow 0}[-2\sin{x}(1-\cos{x})]= -2 x \frac{1}{2}x^2= - x^3 \\
& \therefore  k = 3 \\
\end{aligned}$$

### 填空
>1.
$$\begin{aligned}
& f[\phi(x)] = e^{\phi(x)^2} = 1- x \\
& \phi(x)^2 = ln(1-x) \\
& \phi(x) = \sqrt{\ln{(1-x)}} \\
\end{aligned}$$
>2.
$$\begin{aligned}
& set \quad a_n = \sum_{i=2}^{n} = (1+\frac{2}{n^i})^n \\
& 1+ \frac{2}{n} <  1 + \frac{2}{n} + \frac{2}{n^2} < 1+ \frac{2}{n} + \frac{2}{n(n-1)} \\
& \therefore  1+ \frac{2}{n} < 1 + \frac{2}{n} + \frac{2}{n^2} < 1 + \frac{2}{n-1} \\
& set \quad X_n = \sum_{i=2}^{n} = (1+\frac{2}{n})\\
& set \quad Y_N = \sum_{i=2}^{n} = (1+\frac{2}{n-1}) \\
& \because \lim\limits_{n\rightarrow \infty}(X_n)^n = \lim\limits_{n\rightarrow \infty}(Y_n)^n = e^2 \\
& \therefore \lim\limits_{n\rightarrow \infty}(1 + \frac{2}{n} + \frac{2}{n^2})^n =  e^2 \\
\end{aligned}$$

>3.
$$\begin{aligned}
& 洛:f'(x) = \sin{x} - \sin{a} => \cos{x} - 0 => \cos{x} \\
& g'(x) = x- a  = 1- 0 = 1 \\
& \therefore \lim\limits_{x\rightarrow a} f(x) = \cos{x} \\
\end{aligned}$$

>4.
$$\begin{aligned}
& \because x\rightarrow 0 => \cos{ax}\rightarrow 1 => \ln{\cos{ax}} \rightarrow 0 \\
& \therefore 根据等阶无穷小得=>  \\
& \therefore \lim\limits_{x\rightarrow 0}(\ln{\cos{ax}}) = \lim\limits_{x\rightarrow 0}(\ln{{[ 1 + (\cos{ax} - 1)]}})  =  \lim\limits_{x\rightarrow 0}(\cos{ax} - 1)  \\
&  = \lim\limits_{x\rightarrow 0}- (1-\cos{ax}) = -\frac{1}{2}(ax)^2 \\
& \therefore  = \frac{a^2}{b^2}  \\
\end{aligned}$$

>5.
$$\begin{aligned}
& y=0 => f(0) = f(x)f(0) \\
& \because f(x) \neq  0  \\
& \therefore f(x) = 1 \\
& \therefore f(2008) = 1 \\
\end{aligned}$$

>6.
$$\begin{aligned}
& ??? \\
&  \\
&  \\
\end{aligned}$$

>7.
$$\begin{aligned}
& \lim\limits_{n\rightarrow \infty}\frac{1}{n^2} \ln{[a \cdot a^2 \cdot \dots a^n]}  \\
& \therefore set \quad  a_n = \sum_{i=1}^n = \frac{1}{n^2}\ln{a^i} \\
& \therefore set \quad X_n = \frac{1}{n^2}\ln{a} \\
& set \quad  Y_n = \frac{1}{n^2} \ln{a^{\frac{n(n+1)}{2}}} \\
& \frac{\ln{a^{\frac{n(n+1)}{2}}}}{n^2} = \frac{n(n+1) \ln{a}}{2n^2} = \frac{(n+1)\ln{a}}{2n}\\
& \therefore \lim\limits_{n\rightarrow \infty}Y_n = \lim\limits_{n\rightarrow \infty} \frac{(n+1)\ln{a}}{2n} = \frac{\ln{a}}{2} \\
\end{aligned}$$

>8.
$$\begin{aligned}
& f(x) = f(x+ 5) \\
& f(-1) = f(-1 + 5)  = f(4) = 1 \\
\end{aligned}$$


>9.
$$\begin{aligned}
& \because f(\ln{x}) =x   \\
& \therefore f(x) = e^{x} \\
& \therefore f(3) = e^3 \\
\end{aligned}$$


>10.
$$\begin{aligned}
& if \quad  n > 1 ,then \quad a_n = 2+\frac{1}{a_{n-1}} \\
& \because a_2 > a_3 \\
& \therefore set \quad 2 < a_n < a_{n-1} \\
& \therefore 数列存在 \\
& \lim\limits_{n\rightarrow \infty}a_n = 2 + \frac{1}{\lim\limits_{n\rightarrow \infty}a_{n-1}}   \\
& \because \lim\limits_{n\rightarrow \infty}a_n = \lim\limits_{n\rightarrow \infty}a_{n -1} \\
& \therefore set \quad  a= 2 + \frac{1}{a} => a^2-2a - 1 = 0\\
& \therefore  (a-1)^2 = 2 , a-1 = \pm \sqrt{2} , a= \pm \sqrt{2} + 1 \\
& \therefore a = -\sqrt{2} + 1(舍) a = \sqrt{2} + 1
\end{aligned}$$

简答题
>1.
$$\begin{aligned}
& set \quad f(x) = ax^2 + bx +c  \\
& f(x+1) = a(x+1)^2 + b(x+1) + c = ax^2 + ax + a + bx + b + c \\
& f(x-1) = a(x-1)^2 + b(x-1) + c = ax^2 - ax + a + bx -b + c \\
& f(x+1) + f(x-1) = 2ax^2 + 2a + 2bx +2c = 2x^2 - 4x \\
& \therefore 2a = 2 , 2b = -4 , 2(a+c) = 0 \\
& \therefore a= 1, b = -2,c = -1 \\
& \therefore f(x) = x^2 - 2x -1 = 0
\end{aligned}$$

>2.
$$\begin{aligned}
& 反证 : \\
& \because f(x) = f(x+(2b - 2a)) \\
& \therefore f(b + (-2a + b + x)) = f(b - (-2a + b +x)) = f(2a -x) \\
& =f(  a + (a + x))  = f(a - (a+x)) = f(x)\\
&\therefore 反证成立  \\
\end{aligned}$$

>3.
$$\begin{aligned}
& if \quad x>e: \\
& \ln{(e^n + x^n)} = \ln{[x^n(\frac{e^n}{x^n} + 1)]}  = \ln{x^n} + \ln{[(\frac{e}{x})^2 + 1]}\\
& \because x > e , \therefore \lim\limits_{n\rightarrow \infty}\frac{\ln{x^n} + \ln{[(\frac{e}{x})^2 + 1]}}{n}  = \frac{\ln{x^n}}{n} = \ln{x} \\
& if \quad x<e: \\
& \ln{(e^n + x^n)} = \ln{e^n(1+ \frac{x^n}{e^n})} = n + \ln{(1+\frac{x^n}{e^n})} \\
& \because x<e ,\therefore \lim\limits_{n\rightarrow \infty}\frac{n+\ln{(1+\frac{x^n}{e^n})}}{n} = 1 + \frac{\ln{[1+(\frac{x}{e})^n]}}{n}  = 1 + (\frac{x}{e})^{n-1} = 1\\
& \therefore \lim\limits_{n\rightarrow \infty}f(x) = \begin{cases} &1 , 0<x<e \\ &\ln{x} , x> e \\ \end{cases} \\
\end{aligned}$$

>4.
$$\begin{aligned}
& set \quad g(x) = f(x)  - f(x + \frac{a}{2}) \\
& g(0) = f(0) - f(\frac{a}{2}) \\
& g(\frac{a}{2}) = f(\frac{a}{2}) - f(a) = f(\frac{a}{2}) - f(0) \\
& \therefore g(0) =  - g(\frac{a}{2}) , => f(0) - f(\frac{a}{2}) = f(\frac{a}{2}) - f(a) \\
& if \quad f(0) = f(\frac{a}{2}) \\
& then \quad x = \frac{a}{2} 为(0,a)上的根\\
& if \quad f(0) \neq  f(\frac{a}{2})\\
& then \quad \because g(0) \cdot g(\frac{a}{2}) < 0	 \\
& \therefore 零点定理: set \quad x_0 \in (0,\frac{a}{2}) , 必然有g(x_0) = 0\\
& \therefore 即f(x_0)  - f(x_0 + \frac{a}{2}) = 0\\
& \therefore x_0 是(0,a)内f(x) = f(x + \frac{a}{2})的根\\
\end{aligned}$$


>5.
$$\begin{aligned}
& \because x_1 = \sqrt{2}  > 0 , \therefore x_2 = \sqrt{2 + \sqrt{2} } >  x_1 > 0   \\
& \therefore set \quad \{x_n\}为单调递增的函数 \\
& \because x_n > 0 且 x_n < 2 \\
& \therefore 有界， 则极限存在 \\
& set \quad \lim\limits_{n\rightarrow \infty}x_n = a  \\
& \therefore \lim\limits_{n\rightarrow \infty}x_n = \sqrt{2 + \lim\limits_{n\rightarrow \infty}x_{n- 1}} => a   = \sqrt{2 + a}  \\
& a^2 - a - 2 = 0\\
& (a-2)(a+1) = 0 , a= \begin{cases} &2 \\ &-1(舍) \\ \end{cases}\\
& \\
\end{aligned}$$



<br><br><br><br><br><br><br><br><br><br><br><br><br><br><br><br><br><br><br>

